finish

Property.dfy
@@ -1,81 +1,7 @@
 include "Type.dfy"
 module Property {
   import opened Type
-  // predicate rb_tree_property(root: NodeC?)
-  //   reads root
-  // {
-  //   root_property(root) &&
-  //   red_property(root) &&
-  //   black_property(root)
-
-
-  // }
-
-  // predicate root_property(root: NodeC?)
-  //   reads root
-  // {
-  //   if root == null then true
-  //   else !root.color
-  // }
-
-  // ghost method NodeSize(n: NodeC?) returns (s: nat)
-  //   decreases n
-  // {
-  //   if n == null {
-  //     s := 0;
-  //   } else {
-  //     var l := 0;
-  //     var r := 0;
-  //     l := NodeSize(n.left);
-  //     r := NodeSize(n.right);
-  //     s := 1 + l + r;
-  //   }
-  // }
-
-  // predicate red_property(n: NodeC?)
-  //   reads *
-  //   decreases n
-  // {
-  //   if n == null then true
-  //   else if n.color then
-  //     (n.left == null || !n.left.color) &&
-  //     (n.right == null || !n.right.color) &&
-  //     red_property(n.left) &&
-  //     red_property(n.right)
-  //   else
-  //     red_property(n.left) &&
-  //     red_property(n.right)
-  // }
-
-  // function BlackHeight(n: NodeC?): int
-  //   decreases n
-  // {
-  //   // this implies leaf property
-  //   if n == null then 1
-  //   else
-  //     var left_height := BlackHeight(n.left);
-  //     var right_height := BlackHeight(n.right);
-  //     // We use -1 to show that it is invalid
-  //     if left_height == -1 || right_height == -1 || left_height != right_height then -1
-  //     else left_height + (if n.color then 0 else 1)
-  // }
-
-  // predicate black_property(n: NodeC?) {
-  //   BlackHeight(n) != -1
-  // }
-
-
-  // predicate rb_tree_property_2(t: Rb_tree) {
-  //   match t
-  //   case Null => true
-  //   case Node(_, _, _, _) =>
-  //     root_property2(t) &&
-  //     red_property2(t) &&
-  //     black_property2(t)
-  // }
-
-  // the root node should be black
-  predicate root_property2(t: Rb_tree) {
+  predicate root_property(t: Rb_tree) {
     match t
     case Null => true
     case Node(color, _, _, _) => color == Black
@@ -87,18 +13,6 @@ module Property {
     case Null => Black
     case Node(c, _, _, _) => c
   }
-
-  // // red node cannot have red childrens
-  // predicate red_property2(t: Rb_tree) {
-  //   match t
-  //   case Null => true
-  //   case Node(color, _, left, right) =>
-  //     if color == Red
-  //     then nodeColor(left) == Black &&
-  //          nodeColor(right) == Black &&
-  //          red_property2(left) && red_property2(right)
-  //     else red_property2(left) && red_property2(right)
-  // }
 
   function Max(left:int , right:int):int
   {
@@ -117,10 +31,6 @@ module Property {
       if color == Black then result + 1
       else result
   }
-
-  // predicate black_property2(t: Rb_tree) {
-  //   BlackHeight2(t) != -1
-  // }
 
   function contain(t: Rb_tree) : set<int> {
     match t
@@ -164,11 +74,11 @@ module Property {
   }
 
 
-  predicate isLLRB (t: Rb_tree)
+  predicate strongLLRB (t: Rb_tree)
   {
     match t
     case Null => true
-    case Node(c,k,l,r) => isLLRB(l) && isLLRB(r) && black &&
+    case Node(c,k,l,r) => strongLLRB(l) && strongLLRB(r) && BlackHeight(l) == BlackHeight(r) &&
                           bst_property(t) && goodColor(t)
   }
 
@@ -176,7 +86,7 @@ module Property {
   {
     match t
     case Null => true
-    case Node(c,k,l,r) => isLLRB(l) && isLLRB(r) && black_property2(t) &&
+    case Node(c,k,l,r) => strongLLRB(l) && strongLLRB(r) && BlackHeight(l) == BlackHeight(r) &&
                           bst_property(t) && (nodeColor(r) == Red ==> nodeColor(l) == Red)
   }
 }
